\RequirePackage{plautopatch}
\documentclass[a4paper,11pt]{jsarticle}
\usepackage{color}
\usepackage{subcaption}
\usepackage{listings,jvlisting}
\usepackage{url}
% 数式
\usepackage{amsmath,amsfonts}
\usepackage{bm}
% 画像
\usepackage[dvipdfmx]{graphicx}
\lstset{
  stringstyle={	tfamily},
  commentstyle={	tfamily},
  basicstyle={	tfamily},
  columns=fixed,
  frame={tb},
  breaklines=true,
  columns=[l]{fullflexible},
  numbers=left,%行数を表示したければonにする
  numberstyle={\scriptsize},
  xrightmargin=0em,
  xleftmargin=3em,
  stepnumber=1,
  numbersep=1em,
  tabsize=2,
  lineskip=-0.5ex,
  backgroundcolor=\color{white}
}
\usepackage{geometry}
\geometry{left=25mm,right=25mm,top=20mm,bottom=20mm}
\usepackage{enumitem}
\usepackage{float}
\usepackage{tikz}
\usetikzlibrary{shapes.geometric, arrows,positioning}
\tikzstyle{startstop} = [rectangle, rounded corners, minimum width=3cm, minimum height=1cm,text centered, draw=black, fill=red!20]
\tikzstyle{process0} = [rectangle, minimum width=3cm, minimum height=1cm, text centered, draw=black, fill=red!20]
\tikzstyle{process1} = [rectangle, minimum width=3cm, minimum height=1cm, text centered, draw=black, fill=blue!20]
\tikzstyle{process2} = [rectangle, minimum width=3cm, minimum height=1cm, text centered, draw=black, fill=orange!30]
\tikzstyle{process3} = [rectangle, minimum width=3cm, minimum height=1cm, text centered, draw=black, fill=green!30]
\tikzstyle{arrow} = [thick,->,>=stealth]
\tikzstyle{io} = [trapezium, trapezium left angle=70, trapezium right angle=110, minimum width=3cm, minimum height=1cm, text centered, draw=black, fill=pink!40]
\title{解析学 02課題}
\date{2025-04-16}
\author{橋本 千聡}
\begin{document}
\section*{02-01}\section*{$(1) \int x\sin 2x dx$}
\begin{flalign*}
  &= \int x\left\{-\frac{1}{2}\cos 2x\right\}' dx &&\\
  &= -\frac{1}{2}x\cos 2x - \int -\frac{1}{2}\cos 2x dx &&\\
  &= -\frac{1}{2}x\cos 2x - \frac{1}{4}\sin 2x + C &&
\end{flalign*}

\section*{$(2) \int x\cos 3x dx$}
\begin{flalign*}
  &= \int x\frac{1}{3}\{\sin 3x\}' dx &&\\
  &= \frac{1}{3}x\sin 3x - \int \frac{1}{3}\sin 3x dx &&\\
  &= \frac{1}{3}x\sin 3x + \frac{1}{9}\cos 3x + C &&
\end{flalign*}

\section*{$(3) \int \frac{x}{\cos ^2 x} dx$}
\begin{flalign*}
  &= \int x \{\tan x\}' dx &&\\
  &= x\tan x - \int \tan x dx &&\\
  &= x\tan x - \int \frac{\sin x}{\cos x} dx &&\\
  &= x\tan x - \int \frac{-\{\cos x\}'}{\cos x} dx &&\\
  &= x\tan x - (-\log|\cos x|) + C &&\\
  &= x\tan x + \log|\cos x| + C &&
\end{flalign*}

\section*{$(4) \int x\log(x-2) dx$}
\begin{flalign*}
  &= \int \frac{1}{2}(x^2-2^2)'\log(x-2) &&\\
  &= \frac{1}{2}(x^2-2^2)\log(x-2) - \int \frac{1}{2}(x^2-2^2)\frac{1}{x-2} dx &&\\
  &= \frac{1}{2}(x^2-2^2)\log(x-2) - \int \frac{1}{2}\frac{(x+2)(x-2)}{x-2} dx &&\\
  &= \frac{1}{2}(x^2-2^2)\log(x-2) - \int \frac{1}{2}(x+2) dx &&\\
  &= \frac{1}{2}(x^2-2^2)\log(x-2) - (\frac{1}{4}x^2 + x) + C
\end{flalign*}
\newpage

\section*{$(5) \int x^3\log x dx$}
\begin{flalign*}
  &= \int \frac{1}{4}(x^4)'\log xdx &&\\
  &= \frac{1}{4}x^4\log x - \int \frac{1}{4}x^4\frac{1}{x} dx &&\\
  &= \frac{1}{4}x^4\log x - \int \frac{1}{4}x^3 dx &&\\
  &= \frac{1}{4}x^4\log x - \frac{1}{16}x^4 +C
\end{flalign*}

\section*{$(6) \int (2x-1)e^x dx$}
\begin{flalign*}
  &= \int (2x-1)(e^x)' dx &&\\
  &= (2x-1)e^x - \int 2e^x dx &&\\
  &= (2x-1)e^x - 2e^x + C &&\\
  &= (2x-3)e^x +C
\end{flalign*}

\section*{$(7) \int xe^{-3x}dx$}
\begin{flalign*}
  &= \int -\frac{1}{3} x (e^{-3x})' dx &\\
  &= -\frac{1}{3}xe^{-3x} - \int -\frac{1}{3}e^{-3x} dx &&\\
  &= -\frac{1}{3}xe^{-3x}-\frac{1}{9}e^{-3x} + C &&\\
  &= e^{-3x}(-\frac{1}{3}x -\frac{1}{9})+C &&
\end{flalign*}

\section*{$(8) \int \log(x+2) dx$}
\begin{flalign*}
  &= \int (x+2)'\log(x+2) dx &&\\
  &= (x+2)\log(x+2) - \int (x+2)\frac{1}{x+2} dx &&\\
  &= (x+2)\log(x+2) - \int 1 dx &&\\
  &= (x+2)\log(x+2) -x + C
\end{flalign*}

\newpage

\section*{$(9) \int \log(1-x)dx$}
\begin{flalign*}
  &= \int (x-1)'\log(1-x)dx &&\\
  &= (x-1)\log(1-x) - \int (x-1)\frac{1}{1-x} dx &&\\
  &= (x-1)\log(1-x) - \int -1 dx &&\\
  &= (x-1)\log(1-x) + x +C&&
\end{flalign*}

\section*{02-02}

\section*{$(1) \int x\cos 2xdx$}
\begin{flalign*}
  &= \int \frac{1}{2}x(\sin2x)'dx &&\\
  &= \frac{1}{2}x\sin2x - \int \frac{1}{2}\sin2xdx &&\\
  &= \frac{1}{2}x\sin2x + \frac{1}{4}\cos2x +C
\end{flalign*}

\section*{$(2) \int x\sin3xdx$}
\begin{flalign*}
  &= \int -\frac{1}{3}x(\cos3x)'dx &&\\
  &= -\frac{1}{3}x\cos3x - \int -\frac{1}{3}\cos3x dx &&\\
  &= -\frac{1}{3}x\cos3x + \frac{1}{9}\cos3x + C &&\\
  &= \cos3x(-\frac{1}{3}x + \frac{1}{9}) + C
\end{flalign*}

\section*{$(3) \int \frac{2x}{\cos^2x}dx$}
\begin{flalign*}
  &= \int 2x (\tan x)' dx &&\\
  &=2x\tan x - \int 2\tan xdx &&\\
  &=2x\tan x + 2\log|\cos x| +C
\end{flalign*}

\newpage

\section*{02-03}

\section*{$(1) \int xe^xdx$}
\begin{flalign*}
  &= \int x(e^x)'dx &&\\
  &= xe^x - \int e^x dx &&\\
  &= xe^x - e^x + C &&\\
  &= e^x(x-1) +C
\end{flalign*}

\section*{$(2) \int xe^{-2x}dx$}
\begin{flalign*}
  &= \int -\frac{1}{2}x(e^{-2x})'dx &&\\
  &= -\frac{1}{2}xe^{-2x} - \int -\frac{1}{2}e^{-2x} dx &&\\
  &= -\frac{1}{2}xe^{-2x} - \frac{1}{4}e^{-2x} +C &&\\
  &= e^{-2x}(-\frac{1}{2}x - \frac{1}{4}) +C
\end{flalign*}

\section*{$(3) \int (2x-1)e^{2x}dx$}
\begin{flalign*}
  &= \int \frac{1}{2}(2x-1)(e^{2x})' dx &&\\
  &= \frac{1}{2}(2x-1)e^{2x} - \int e^{2x}dx &&\\
  &= \frac{1}{2}(2x-1)e^{2x} - 2e^{2x} +C&&\\
  &= e^{2x}(x-\frac{5}{2}) +C
\end{flalign*}

\section*{$(4) \int x^2\log xdx$}
\begin{flalign*}
  &= \int \frac{1}{3}(x^3)'\log x dx &&\\
  &= \frac{1}{3}x^3\log x - \int \frac{1}{3}x^3\frac{1}{x} dx &&\\
  &= \frac{1}{3}x^3\log x - \frac{1}{9}x^3 +C &&\\
\end{flalign*}

\newpage

\section*{$(5) \int (x-1)^3\log(x-1)dx$}
\begin{flalign*}
  &= \int \frac{1}{4}\{(x-1)^4\}'\log(x-1)dx &&\\
  &= \frac{1}{4}(x-1)^4\log(x-1) - \int \frac{1}{4}(x-1)^4\frac{1}{x-1}dx &&\\
  &= \frac{1}{4}(x-1)^4\log(x-1) - \frac{1}{16}(x-1)^4 +C &&\\
\end{flalign*}

\section*{$(6) \int \log 2xdx$}
\begin{flalign*}
  &= \int \frac{1}{2}(2x)'\log2xdx &&\\
  &= x\log2x - \int \frac{1}{2}2x\frac{1}{2x} dx &&\\
  &= x\log2x - \frac{1}{2}x +C  
\end{flalign*}

\section*{$(7) \int \log(3-x)dx$}
\begin{flalign*}
  &= \int (x-3)'\log(3-x)dx&&\\
  &= (x-3)\log(3-x) - \int (x-3)\frac{1}{3-x} dx &&\\
  &=
\end{flalign*}

\section*{02-04}
\section*{$(1) \int x^2\sin xdx$}
\begin{flalign*}
  &= \int x^2(-\cos x)'dx &&\\
  &= -x^2\cos x - \int -2x\cos x dx &&\\
  &= -x^2\cos x - \int -2x(\sin x)' dx &&\\
  &= -x^2\cos x - (-2x\sin x - \int -2\sin x dx) &&\\
  &= -x^2\cos x +x2\sin x-2\sin x + C
\end{flalign*}

\section*{$(2) \int x^2e^{-x}dx$}
\begin{flalign*}
  &= \int -x^2(e^{-x})'dx &&\\
  &= -x^2e^{-x} - \int -2xe^{-x}dx &&\\
  &= -x^2e^{-x} - \int 2xe^{-x}dx &&\\
  &= -x^2e^{-x} - (2xe^{-x} - \int 2e^{-x}dx)&&\\
  &= -x^2e^{-x} - 2xe^{-x} - 2e^{-x} +C
\end{flalign*}

\end{document}