\RequirePackage{plautopatch}
\documentclass[a4paper,11pt]{jsarticle}
\usepackage{color}
\usepackage{subcaption}
\usepackage{listings,jvlisting}
\usepackage{url}
\usepackage{multicol}
% 数式
\usepackage{amsmath,amsfonts}
\usepackage{bm}
% 画像
\usepackage[dvipdfmx]{graphicx}
\lstset{
  stringstyle={	tfamily},
  commentstyle={	tfamily},
  basicstyle={	tfamily},
  columns=fixed,
  frame={tb},
  breaklines=true,
  columns=[l]{fullflexible},
  numbers=left,%行数を表示したければonにする
  numberstyle={\scriptsize},
  xrightmargin=0em,
  xleftmargin=3em,
  stepnumber=1,
  numbersep=1em,
  tabsize=2,
  lineskip=-0.5ex,
  backgroundcolor=\color{white}
}
\usepackage{geometry}
\geometry{left=25mm,right=25mm,top=20mm,bottom=20mm}
\usepackage{enumitem}
\title{解析学05 定積分}
\date{2025/05/13}
\author{3I 31 橋本 千聡}
\begin{document}
\maketitle
\begin{multicols}{2}

\section*{5-1}
\section*{$ (1) f(x) = \int_{1}^{x-3}(x-3-p)\log p dp $}
\noindent
\begin{flalign*}
  f(x) &= \int_{1}^{x-3}(x-3-p)\log p dp &&\\
  &= \int_{1}^{x-3} (x-3)\log p - p\log p dp \\
  &= (x-3) \int_{1}^{x-3} \log p dp - \int_{1}^{x-3} p\log p dp \\
 \frac{df(x)}{dx} &= [p\log p - p]_{1}^{x-3} \\
  &= (x-3)\log(x-3) -x +4
\end{flalign*}

\section*{$ (2) g(x) = -\int_{0}^{x^2}(x^2-s)e^sds$}
\noindent
\begin{flalign*}
  g(x) &= -x^2\int_{0}^{x^2} e^sds + \int_{0}^{x^2} se^s ds &&\\
  \frac{dg(x)}{dx} &= 2x(-\int_{0}^{x^2} e^sds - x^2e^{x^2} + x^2e^{x^2}) \\
  &= 2x(1-e^{x^2})
\end{flalign*}

\section*{5-2}
\section*{$ (1) \int_1^3 4x^3dx$}
\noindent
\begin{flalign*}
  &= [x^4]_1^3 &&\\
  &= 3^4-1^4 &&\\
  &=80
\end{flalign*}

\section*{$ (2) \int_1^4\sqrt x dx$}
\noindent
\begin{flalign*}
  &= [\frac23x^\frac32]_1^4 &&\\
  &= \frac23 4\sqrt4 - \frac23 &&\\
  &= \frac{14}3
\end{flalign*}

\section*{$ (3) \int_1^4 x^{-\frac32}dx$}
\noindent
\begin{flalign*}
  &=[-2x^{-\frac{1}{2}}]_1^4 &&\\
  &= -2\frac{1}{\sqrt4} - 2&&\\
  &= -3
\end{flalign*}

\section*{$ (4) \int_e^{e^2}\frac{dx}{x}$}
\noindent
\begin{flalign*}
  &=[\log |x|]_e^{e+1}&&\\
  &= 2-1 &&\\
  &= 1
\end{flalign*}

\section*{$ (5) \int_2^{e+1}\frac{dy}{1-y}$}
\noindent
\begin{flalign*}
  &=[-\log |1-y|]_2^{e+1} &&\\
  &=  -1 + 0 &&\\
  &= -1
\end{flalign*}

\section*{$ (6) \int_0^\pi \sin\theta d\theta$}
\noindent
\begin{flalign*}
  &= [-\cos \theta]_0^\pi &&\\
  &=  -0 -1 &&\\
  &= 1
\end{flalign*}

\section*{$ (7) \int_-{\frac\pi2}^{\frac\pi2} \cos tdt$}
\noindent
\begin{flalign*}
  &=2\int_0^1\cos tdt&&\\
  &= 2[\sin t]_0^1 &&\\
  &= 2
\end{flalign*}

\section*{$ (8) \int_0^{\log2} e^{3x}dx$}
\noindent
\begin{flalign*}
  &=[\frac13 e^{3x}]_0^{\log 2}&&\\
  &= \frac13 e^{3\log2} - \frac13 &&\\
  &= \frac{7}{3}
\end{flalign*}

\section*{$ (9) \int_1^2 2^xdx $}
\noindent
\begin{flalign*}
  &=[\frac{2^x}{\log2}]_1^2 &&\\
  &= \frac{2}{\log2}
\end{flalign*}

\section*{05-03}
\section*{$ (1) \int_0^{\frac\pi2}(\sin2x+\cos3x)dx$}
\noindent
\begin{flalign*}
  &=[-\frac12 \cos2x +\frac13\sin3x]_0^\frac\pi2&&\\
  &= (\frac12-\frac13)-(-\frac12+0) &&\\
  &=\frac23
\end{flalign*}

\section*{$ (2) \int_\pi t^3\pi \cos(\frac{x}4-\frac\pi4)dx$}
\noindent
\begin{flalign*}
  &= [4\sin(\frac{x}{4}-\frac{\pi}{4})]_0^{\frac{\pi}{2}} &&\\
  &= 4-0 &&\\
  &= 4
\end{flalign*}

\section*{$ (3) \int_1^2\sin(\frac23 \pi t+\frac\pi4)dt $}
\noindent
\begin{flalign*}
  &=[-\frac{3}{2\pi}\cos(\frac23\pi t+\frac\pi4)]_1^2 &&\\
  &= -\frac3{2\pi}(\cos\frac{19}{12}\pi - \cos\frac{11}{12}\pi) &&
\end{flalign*}

\section*{$ (4) \int_0^{\frac\pi4}\cos^2x dx $}
\noindent
\begin{flalign*}
  &=\int_0^{\frac\pi4}\frac12(1+\cos2x)dx&&\\
  &= \frac12[x+\frac12\sin2x]_0^{\frac\pi4} &&\\
  &= \frac{\pi+\sqrt2}{8}
\end{flalign*}

\section*{$ (5) \int_0^\frac\pi8 \sin^2 2xdx$}
\noindent
\begin{flalign*}
  &=\int_0^{\frac\pi8}\frac12(1-\cos4x)dx&&\\
  &= \frac12[x-\frac14\sin4\pi]_0^{\frac\pi8} &&\\
  &= \frac{\pi-\sqrt2}{16}
\end{flalign*}

\section*{$ (6) \int_0^\frac\pi4 \tan^2xdx$}
\noindent
\begin{flalign*}
  &=\int_0^{\frac\pi4}(\frac{1}{\cos^2x}-1)dx&&\\
  &= [\tan x -x]_0^{\frac\pi4} &&\\
  &= 1-\frac{\pi}{4} &&
\end{flalign*}

\section*{05-04}
\section*{$ (1) \int_0^2 x(x^2+1)^3 dx$}
\noindent
\begin{flalign*}
  t&=x^2+1 &&\\
  dt&=2xdx &&\\
  I&=\frac12\int_1^5 t^3 dt &&\\
  &= \frac{624}{8} &&\\
\end{flalign*}

\section*{$ (2) \int_1^2 \frac{x^2-2x}{x^3-3x^2+1}dx$}
\noindent
\begin{flalign*}
  &= [\frac13\log|x^3-3x^2+1|]_1^2 &&\\
  &= \frac{1}{3}\log3
\end{flalign*}

\end{multicols}
\end{document}